SystemFD/Algorithm/TypeMatch.lean
@@ -37,74 +37,110 @@ theorem stable_type_match_sound_lemma :
   .some (x, sp) = Term.neutral_form R ->
   (Γ d@ x).is_stable ->
   StableTypeMatch Γ A R
-:= by sorry
--- intro h1 h2 h3 h4
--- induction A generalizing τ sR R x sp Γ <;> try simp at h1
--- any_goals try (
---   case _ =>
---     cases h1; case _ e1 e2 =>
---       subst e1; subst e2
---       simp at h2; subst h2; constructor
---       apply h3; apply h4
--- )
--- case _ => sorry
--- case _ v t1 t2 ih1 ih2 =>
---   sorry
---   -- cases v <;> try simp at h1
---   -- any_goals try (
---   --   case _ =>
---   --     cases h1; case _ e1 e2 =>
---   --       subst e1; subst e2
---   --       simp at h2; subst h2; constructor
---   --       apply h3; apply h4
---   -- )
---   case all =>
---     cases τ
---     case _ => simp at h1
---     case _ hd τ =>
---       have lem1 : (τ, sR) = t2.to_telescope := by
---         cases h1; case _ u1 u2 =>
---           subst u2; injection u1 with _ e; subst e
---           generalize zdef : t2.to_telescope = z
---           apply Prod.eta
---       have lem2 : [S' τ.length][S]R = sR := by simp at h2; simp [*]
---       have lem3 :
---         .some (x + 1, List.map (λ (v, t) => (v, [S]t)) sp)
---         = ([S]R).neutral_form
---       := by
---         replace h3 := Eq.symm h3
---         have lem := neutral_form_rename (fun x => x + 1) h3
---         rw [Subst.to_S] at lem; rw [lem]; simp
---       have lem4 : ((Frame.kind t1 :: Γ)d@(x + 1)).is_stable := by
---         simp; rw [Frame.is_stable_stable]; apply h4
---       simp at h2; constructor
---       apply ih2 lem1 lem2 lem3 lem4
---   case arrow =>
---     cases τ
---     case _ => simp at h1
---     case _ hd τ =>
---       have lem1 : (τ, sR) = t2.to_telescope := by
---         cases h1; case _ u1 u2 =>
---           subst u2; injection u1 with _ e; subst e
---           generalize zdef : t2.to_telescope = z
---           apply Prod.eta
---       have lem2 : [S' τ.length][S]R = sR := by simp at h2; simp [*]
---       have lem3 :
---         .some (x + 1, List.map (λ (v, t) => (v, [S]t)) sp)
---         = ([S]R).neutral_form
---       := by
---         replace h3 := Eq.symm h3
---         have lem := neutral_form_rename (fun x => x + 1) h3
---         rw [Subst.to_S] at lem; rw [lem]; simp
---       have lem4 : ((Frame.type t1 :: Γ)d@(x + 1)).is_stable := by
---         simp; rw [Frame.is_stable_stable]; apply h4
---       simp at h2; constructor
---       apply ih2 lem1 lem2 lem3 lem4
+:= by
+intro h1 h2 h3 h4
+induction A generalizing τ sR R x sp Γ <;> try simp at h1
+any_goals try (
+  case _ =>
+    cases h1; case _ e1 e2 =>
+      subst e1; subst e2
+      simp at h2; subst h2; constructor
+      unfold ValidHeadVariable;
+      apply Exists.intro _; apply And.intro
+      apply h3; apply h4
+)
+case _ v t1 t2 ih1 ih2 =>
+  cases v <;> try simp at h1
+  any_goals try (
+    case _ =>
+      cases h1; case _ e1 e2 =>
+        subst e1; subst e2
+        simp at h2; subst h2; constructor
+        unfold ValidHeadVariable;
+        apply Exists.intro _; apply And.intro
+        apply h3; apply h4
+  )
+  case all =>
+    cases τ
+    case _ => simp at h1
+    case _ hd τ =>
+      have lem1 : (τ, sR) = t2.to_telescope := by
+        cases h1; case _ u1 u2 =>
+          subst u2; injection u1 with _ e; subst e
+          generalize zdef : t2.to_telescope = z
+          apply Prod.eta
+      have lem2 : [S' τ.length][S]R = sR := by simp at h2; simp [*]
+      have lem3 :
+        .some (x + 1, List.map (λ (v, t) => (v, [S]t)) sp)
+        = ([S]R).neutral_form
+      := by
+        replace h3 := Eq.symm h3
+        have lem := neutral_form_rename (fun x => x + 1) h3
+        rw [Subst.to_S] at lem; rw [lem]; simp
+      have lem4 : ((Frame.kind t1 :: Γ)d@(x + 1)).is_stable := by
+        simp; rw [Frame.is_stable_stable]; apply h4
+      apply StableTypeMatch.all
+      case _ =>
+        simp at *; unfold ValidHeadVariable
+        have lem5 : @Ren.to Term (· - 1) = P := by
+          unfold Ren.to; unfold P; simp
+        have lem6 := neutral_form_rename (· - 1) (Eq.symm lem3)
+        rw [lem5] at lem6; simp at lem6
+        rw [Frame.is_stable_stable] at lem4
+        unfold Function.comp at lem6; simp at lem6
+        apply Exists.intro (x, sp)
+        apply And.intro (Eq.symm lem6); simp
+        apply lem4
+      case _ => apply ih2 lem1 lem2 lem3 lem4
+  case arrow =>
+    cases τ
+    case _ => simp at h1
+    case _ hd τ =>
+      have lem1 : (τ, sR) = t2.to_telescope := by
+        cases h1; case _ u1 u2 =>
+          subst u2; injection u1 with _ e; subst e
+          generalize zdef : t2.to_telescope = z
+          apply Prod.eta
+      have lem2 : [S' τ.length][S]R = sR := by simp at h2; simp [*]
+      have lem3 :
+        .some (x + 1, List.map (λ (v, t) => (v, [S]t)) sp)
+        = ([S]R).neutral_form
+      := by
+        replace h3 := Eq.symm h3
+        have lem := neutral_form_rename (fun x => x + 1) h3
+        rw [Subst.to_S] at lem; rw [lem]; simp
+      have lem4 : ((Frame.type t1 :: Γ)d@(x + 1)).is_stable := by
+        simp; rw [Frame.is_stable_stable]; apply h4
+      apply StableTypeMatch.arrow
+      case _ =>
+        simp at *; unfold ValidHeadVariable
+        have lem5 : @Ren.to Term (· - 1) = P := by
+          unfold Ren.to; unfold P; simp
+        have lem6 := neutral_form_rename (· - 1) (Eq.symm lem3)
+        rw [lem5] at lem6; simp at lem6
+        rw [Frame.is_stable_stable] at lem4
+        unfold Function.comp at lem6; simp at lem6
+        apply Exists.intro (x, sp)
+        apply And.intro (Eq.symm lem6); simp
+        apply lem4
+      case _ => apply ih2 lem1 lem2 lem3 lem4
 
 theorem stable_type_match_sound :
   stable_type_match Γ A R = .some u ->
   StableTypeMatch Γ A R
-:= by sorry
+:= by
+intro h
+unfold stable_type_match at h
+simp at h; rw [Option.bind_eq_some] at h; simp at h
+cases h; case _ a h =>
+cases h; case _ h1 h2 =>
+cases h1; case _ sp h1 =>
+cases h2; case _ h2 h3 =>
+  generalize sRdef : A.to_telescope = Asp at *
+  cases Asp; case _ τ sR =>
+    replace h2 := Term.eq_of_beq h2; simp at *
+    apply stable_type_match_sound_lemma
+      (Eq.symm sRdef) h2 (Eq.symm h1) h3
 
 theorem telescope_empty {B : Term} :
   ([], sB) = B.to_telescope ->
@@ -258,29 +294,201 @@ theorem prefix_type_match_sound :
   PrefixTypeMatch Γ A B T
 := by
 intros h;
-unfold prefix_type_match at h; simp at h;
-rw[Option.bind_eq_some] at h;
-cases h; case _ u1 h1 =>
-cases h1; case _ u2 h1 =>
-rw[Option.bind_eq_some] at h1;
-cases h1; case _ u1 h1 =>
-cases h1; case _ u1 h1 =>
-simp at h1;
-have h2 := h1.1.1.1;
-have h3 := h1.1.1.2;
-have h4 := h1.1.2;
-have h5 := h1.2;
- sorry
+unfold prefix_type_match at h; simp at h
+rw [Option.bind_eq_some] at h
+cases h; case _ ξ h =>
+cases h; case _ h1 h2 =>
+rw [Option.bind_eq_some] at h2; simp at h2
+cases h2; case _ x h2 =>
+cases h2; case _ h2 h3 =>
+cases h3; case _ h3 h4 =>
+cases h3; case _ h3 h5 =>
+cases h3; case _ h3 h6 =>
+cases h2; case _ sp h2 =>
+  generalize Aspdef : A.to_telescope = Asp at *
+  generalize Bspdef : B.to_telescope = Bsp at *
+  cases Asp; case _ τ sR =>
+  cases Bsp; case _ τ' sT =>
+    simp at *
+    replace h6 := Term.eq_of_beq h6
+    replace h3 := Term.eq_of_beq h3
+    apply prefix_type_match_sound_lemma
+      (Eq.symm Aspdef) (Eq.symm Bspdef) (Eq.symm h1)
+    rw [<-h4]; simp; apply h3
+    rw [<-Subst.apply_compose_commute] at h6
+    apply h6; apply Eq.symm h2
+    apply h5
 
+theorem valid_ctor_sound_lemma :
+  (τ, sR) = Term.to_telescope A ->
+  [S' τ.length]R = sR ->
+  .some (x, sp) = Term.neutral_form R ->
+  (Γ d@ x).is_datatype ->
+  ValidCtor Γ A
+:= by
+intro h1 h2 h3 h4
+induction A generalizing τ sR R x sp Γ <;> try simp at h1
+any_goals try (
+  case _ =>
+    cases h1; case _ e1 e2 =>
+      subst e1; subst e2
+      simp at h2; subst h2; constructor
+      unfold ValidHeadVariable;
+      apply Exists.intro _; apply And.intro
+      apply h3; apply h4
+)
+case _ v t1 t2 ih1 ih2 =>
+  cases v <;> try simp at h1
+  any_goals try (
+    case _ =>
+      cases h1; case _ e1 e2 =>
+        subst e1; subst e2
+        simp at h2; subst h2; constructor
+        unfold ValidHeadVariable;
+        apply Exists.intro _; apply And.intro
+        apply h3; apply h4
+  )
+  case all =>
+    cases τ
+    case _ => simp at h1
+    case _ hd τ =>
+      have lem1 : (τ, sR) = t2.to_telescope := by
+        cases h1; case _ u1 u2 =>
+          subst u2; injection u1 with _ e; subst e
+          generalize zdef : t2.to_telescope = z
+          apply Prod.eta
+      have lem2 : [S' τ.length][S]R = sR := by simp at h2; simp [*]
+      have lem3 :
+        .some (x + 1, List.map (λ (v, t) => (v, [S]t)) sp)
+        = ([S]R).neutral_form
+      := by
+        replace h3 := Eq.symm h3
+        have lem := neutral_form_rename (fun x => x + 1) h3
+        rw [Subst.to_S] at lem; rw [lem]; simp
+      have lem4 : ((Frame.kind t1 :: Γ)d@(x + 1)).is_datatype := by
+        simp; rw [Frame.is_datatype_stable]; apply h4
+      apply ValidCtor.all
+      apply ih2 lem1 lem2 lem3 lem4
+  case arrow =>
+    cases τ
+    case _ => simp at h1
+    case _ hd τ =>
+      have lem1 : (τ, sR) = t2.to_telescope := by
+        cases h1; case _ u1 u2 =>
+          subst u2; injection u1 with _ e; subst e
+          generalize zdef : t2.to_telescope = z
+          apply Prod.eta
+      have lem2 : [S' τ.length][S]R = sR := by simp at h2; simp [*]
+      have lem3 :
+        .some (x + 1, List.map (λ (v, t) => (v, [S]t)) sp)
+        = ([S]R).neutral_form
+      := by
+        replace h3 := Eq.symm h3
+        have lem := neutral_form_rename (fun x => x + 1) h3
+        rw [Subst.to_S] at lem; rw [lem]; simp
+      have lem4 : ((Frame.type t1 :: Γ)d@(x + 1)).is_datatype := by
+        simp; rw [Frame.is_datatype_stable]; apply h4
+      apply ValidCtor.arrow
+      apply ih2 lem1 lem2 lem3 lem4
 
 theorem valid_ctor_sound : valid_ctor Γ A = .some () -> ValidCtor Γ A := by
-intros h;
-unfold valid_ctor at h; split at h;
-case _ τ sA tele =>
-simp at h;
-rw[Option.bind_eq_some] at h;
-cases h; case _ w h =>
-simp at h;
+intro h
+unfold valid_ctor at h; simp at h
+rw [Option.bind_eq_some] at h; simp at h
+cases h; case _ a h =>
+cases h; case _ h1 h2 =>
+cases h2; case _ h2 h3 =>
+cases h1; case _ sp h1 =>
+  generalize Aspdef : A.to_telescope = Asp at *
+  cases Asp; case _ τ sR =>
+    simp at *; replace h2 := Term.eq_of_beq h2
+    rw [<-Subst.apply_compose_commute] at h2
+    apply valid_ctor_sound_lemma
+      (Eq.symm Aspdef) h2 (Eq.symm h1) h3
 
- sorry
-theorem valid_insttype_sound : valid_insttype Γ A = .some () -> ValidInstType Γ A := by sorry
+theorem valid_insttype_sound_lemma :
+  (τ, sR) = Term.to_telescope A ->
+  [S' τ.length]R = sR ->
+  .some (x, sp) = Term.neutral_form R ->
+  (Γ d@ x).is_opent ->
+  ValidInstType Γ A
+:= by
+intro h1 h2 h3 h4
+induction A generalizing τ sR R x sp Γ <;> try simp at h1
+any_goals try (
+  case _ =>
+    cases h1; case _ e1 e2 =>
+      subst e1; subst e2
+      simp at h2; subst h2; constructor
+      unfold ValidHeadVariable;
+      apply Exists.intro _; apply And.intro
+      apply h3; apply h4
+)
+case _ v t1 t2 ih1 ih2 =>
+  cases v <;> try simp at h1
+  any_goals try (
+    case _ =>
+      cases h1; case _ e1 e2 =>
+        subst e1; subst e2
+        simp at h2; subst h2; constructor
+        unfold ValidHeadVariable;
+        apply Exists.intro _; apply And.intro
+        apply h3; apply h4
+  )
+  case all =>
+    cases τ
+    case _ => simp at h1
+    case _ hd τ =>
+      have lem1 : (τ, sR) = t2.to_telescope := by
+        cases h1; case _ u1 u2 =>
+          subst u2; injection u1 with _ e; subst e
+          generalize zdef : t2.to_telescope = z
+          apply Prod.eta
+      have lem2 : [S' τ.length][S]R = sR := by simp at h2; simp [*]
+      have lem3 :
+        .some (x + 1, List.map (λ (v, t) => (v, [S]t)) sp)
+        = ([S]R).neutral_form
+      := by
+        replace h3 := Eq.symm h3
+        have lem := neutral_form_rename (fun x => x + 1) h3
+        rw [Subst.to_S] at lem; rw [lem]; simp
+      have lem4 : ((Frame.kind t1 :: Γ)d@(x + 1)).is_opent := by
+        simp; rw [Frame.is_opent_stable]; apply h4
+      apply ValidInstType.all
+      apply ih2 lem1 lem2 lem3 lem4
+  case arrow =>
+    cases τ
+    case _ => simp at h1
+    case _ hd τ =>
+      have lem1 : (τ, sR) = t2.to_telescope := by
+        cases h1; case _ u1 u2 =>
+          subst u2; injection u1 with _ e; subst e
+          generalize zdef : t2.to_telescope = z
+          apply Prod.eta
+      have lem2 : [S' τ.length][S]R = sR := by simp at h2; simp [*]
+      have lem3 :
+        .some (x + 1, List.map (λ (v, t) => (v, [S]t)) sp)
+        = ([S]R).neutral_form
+      := by
+        replace h3 := Eq.symm h3
+        have lem := neutral_form_rename (fun x => x + 1) h3
+        rw [Subst.to_S] at lem; rw [lem]; simp
+      have lem4 : ((Frame.type t1 :: Γ)d@(x + 1)).is_opent := by
+        simp; rw [Frame.is_opent_stable]; apply h4
+      apply ValidInstType.arrow
+      apply ih2 lem1 lem2 lem3 lem4
+
+theorem valid_insttype_sound : valid_insttype Γ A = .some () -> ValidInstType Γ A := by
+intro h
+unfold valid_insttype at h; simp at h
+rw [Option.bind_eq_some] at h; simp at h
+cases h; case _ a h =>
+cases h; case _ h1 h2 =>
+cases h2; case _ h2 h3 =>
+cases h1; case _ sp h1 =>
+  generalize Aspdef : A.to_telescope = Asp at *
+  cases Asp; case _ τ sR =>
+    simp at *; replace h2 := Term.eq_of_beq h2
+    rw [<-Subst.apply_compose_commute] at h2
+    apply valid_insttype_sound_lemma
+      (Eq.symm Aspdef) h2 (Eq.symm h1) h3
